alloc_metadata 13/n: extraction working, done

src/ffs.c
@@ -1,10 +1,20 @@
 #include <stddef.h>
 #include <stdint.h>
 //#include <stdio.h>
+//
+#include "Slabs.h"
 
 uint32_t Utils2_ffs64(uint64_t x) {
   return __builtin_ffsll(~x);
 }
+
+
+Selectors_LList_cell__Slabs_blob
+*Slabs_singleton_array_to_ref(Selectors_LList_cell__Slabs_blob *arr) {
+  return arr;
+}
+
+
 
 //int main(){
 //  uint64_t v;
