src/SizeClass.fst
@@ -4,40 +4,37 @@ module U64 = FStar.UInt64
 module U32 = FStar.UInt32
 module U8 = FStar.UInt8
 
-module G =  FStar.Ghost
+module G = FStar.Ghost
 
 module SL = Selectors.LList
 
-open Steel.FractionalPermission
-module Mem = Steel.Memory
+module P = Steel.FractionalPermission
+module SM = Steel.Memory
+module A = Steel.Array
+
 open Steel.Effect.Atomic
 open Steel.Effect
 open Steel.Reference
-module SR = Steel.Reference
-module A = Steel.Array
-module P = Steel.FractionalPermission
 
 open Utils2
 open Slabs
 
-//TODO: use ptrdiff
-//assume val f (md: slab_metadata) : arr:array U8.t{A.length arr = U32.v page_size}
+#push-options "--ide_id_info_off"
 
-// Given a size, return a size_class
-// TODO: improve max_sc bound
-// (requires an improved Steel while loop)
+//TODO: remove blob, use ptrdiff style
+//TODO: improve max_sc bound, use better spec'ed ffs64
 
-
+open FStar.Mul
 noeq
 type size_class_struct = {
   size: sc;
   partial_slabs: ref (SL.t blob);
   empty_slabs: ref (SL.t blob);
   md_count: ref U32.t;
-  slab_region: array U8.t;
+  slab_region: slab_region:array U8.t{A.length slab_region = U32.v metadata_max * U32.v page_size};
   //TODO: duplicata due to karamel extraction issue
-  md_bm_region: array U64.t;
-  md_region: array (SL.cell blob);
+  md_bm_region: md_bm_region:array U64.t{A.length md_bm_region = U32.v metadata_max * 4};
+  md_region: md_region:array (SL.cell blob){A.length md_region = U32.v metadata_max};
   //lock: ref bool;
 }
 
@@ -52,490 +49,56 @@ type blob2 = {
   md_region_v: Seq.seq (SL.cell blob);
 }
 
-let size_class_sl'
-  (r: ref size_class_struct)
+open SteelVRefineDep
+
+let size_class_vprop_aux
   (scs: size_class_struct)
-  : Mem.slprop u#1
+  : vprop
   =
-  pts_to_sl r full_perm scs `Mem.star`
-  SL.ind_llist_sl (p_partial scs.size) (scs.partial_slabs) `Mem.star`
-  SL.ind_llist_sl (p_empty scs.size) (scs.empty_slabs) `Mem.star`
-  hp_of (A.varray scs.slab_region) `Mem.star`
-  hp_of (A.varray scs.md_bm_region) `Mem.star`
-  hp_of (A.varray scs.md_region) `Mem.star`
-  hp_of (vptr scs.md_count)
-
-let size_class_sl
-  (r: ref size_class_struct)
-  =
-  Mem.h_exists (size_class_sl' r)
-
-let size_class_sl'_witinv (r: ref size_class_struct)
-  : Lemma (Mem.is_witness_invariant (size_class_sl' r))
-  =
-  let aux (scs1 scs2: size_class_struct) (m: Mem.mem)
-  : Lemma
-  (requires
-    Mem.interp (size_class_sl' r scs1) m /\
-    Mem.interp (size_class_sl' r scs2) m
-  )
-  (ensures scs1 == scs2)
-  =
-  pts_to_witinv r full_perm;
-  assert (scs1 == scs2)
-  in
-  Classical.forall_intro_3 (Classical.move_requires_3 aux)
-
-let size_class_sel_full'
-  (r: ref size_class_struct)
-  : selector' blob2 (size_class_sl r)
-  =
-  fun (h:_) ->
-    let scs : size_class_struct = G.reveal (Mem.id_elim_exists (size_class_sl' r) h) in
-    assert (Mem.interp (size_class_sl' r scs) h);
-    let p1 = pts_to_sl r full_perm scs in
-    let p2 = SL.ind_llist_sl (p_partial scs.size) scs.partial_slabs in
-    let p3 = SL.ind_llist_sl (p_empty scs.size) scs.empty_slabs in
-    let p4 = hp_of (A.varray scs.slab_region) in
-    let p5 = hp_of (A.varray scs.md_bm_region) in
-    let p6 = hp_of (A.varray scs.md_region) in
-    let p7 = SR.ptr scs.md_count in
-    let sl =
-      p1 `Mem.star` p2 `Mem.star` p3 `Mem.star`
-      p4 `Mem.star` p5 `Mem.star` p6 `Mem.star`
-      p7 in
-    assert (Mem.interp sl h);
-    let partial_slabs_v = SL.ind_llist_sel (p_partial scs.size) scs.partial_slabs h in
-    let empty_slabs_v = SL.ind_llist_sel (p_empty scs.size) scs.empty_slabs h in
-    let slab_region_v = A.varrayp_sel scs.slab_region P.full_perm h in
-    let md_bm_region_v = A.varrayp_sel scs.md_bm_region P.full_perm h in
-    let md_region_v = A.varrayp_sel scs.md_region P.full_perm h in
-    let md_count_v = SR.ptrp_sel scs.md_count P.full_perm h in
-    let b = {
-      scs_v = G.reveal scs;
-      partial_slabs_v = partial_slabs_v;
-      empty_slabs_v = empty_slabs_v;
-      md_count_v = md_count_v;
-      slab_region_v = slab_region_v;
-      md_bm_region_v = md_bm_region_v;
-      md_region_v = md_region_v;
-    } in
-    b
-
-let size_class_sel_depends_only_on
-  (r: ref size_class_struct)
-  (m0:Mem.hmem (size_class_sl r)) (m1:Mem.mem{Mem.disjoint m0 m1})
-  : Lemma
-  (size_class_sel_full' r m0 == size_class_sel_full' r (Mem.join m0 m1))
-  =
-  let m' = Mem.join m0 m1 in
-  let b1 = G.reveal (Mem.id_elim_exists (size_class_sl' r) m0) in
-  let b2 = G.reveal (Mem.id_elim_exists (size_class_sl' r) m') in
-  size_class_sl'_witinv r;
-  Mem.elim_wi (size_class_sl' r) b1 b2 m'
-
-let size_class_sel_depends_only_on_core
-  (r: ref size_class_struct)
-  (m0:Mem.hmem (size_class_sl r))
-  : Lemma
-  (size_class_sel_full' r m0 == size_class_sel_full' r (Mem.core_mem m0))
-  =
-  let b1 = G.reveal (Mem.id_elim_exists (size_class_sl' r) m0) in
-  let b2 = G.reveal (Mem.id_elim_exists (size_class_sl' r) (Mem.core_mem m0)) in
-  size_class_sl'_witinv r;
-  Mem.elim_wi (size_class_sl' r) b1 b2 (Mem.core_mem m0)
-
-let size_class_sel (r: ref size_class_struct)
-  : selector blob2 (size_class_sl r)
-  =
-  Classical.forall_intro_2 (size_class_sel_depends_only_on r);
-  Classical.forall_intro (size_class_sel_depends_only_on_core r);
-  size_class_sel_full' r
-
-[@@ __steel_reduce__]
-let size_class_full' (r: ref size_class_struct) : vprop'
-  = {
-    hp = size_class_sl r;
-    t = blob2;
-    sel = size_class_sel r;
-  }
-//TODO: FIXME: extracts despite noextract qualifier
-unfold
-noextract
-let size_class_full (r: ref size_class_struct) = VUnit (size_class_full' r)
-
-[@@ __steel_reduce__]
-let v_sc_full (#p: vprop) (r: ref size_class_struct)
-  (h: rmem p{FStar.Tactics.with_tactic selector_tactic (can_be_split p (size_class_full r) /\ True)})
-  = h (size_class_full r)
-
-let unpack_sc_lemma
-  (r: ref size_class_struct)
-  (b: blob2)
-  (m: Mem.mem)
-  : Lemma
-  (requires
-    Mem.interp (size_class_sl r) m /\
-    size_class_sel r m == b
-  )
-  (ensures (
-    Mem.interp (
-      SR.ptr r `Mem.star`
-      SL.ind_llist_sl (p_partial b.scs_v.size) b.scs_v.partial_slabs `Mem.star`
-      SL.ind_llist_sl (p_empty b.scs_v.size) b.scs_v.empty_slabs `Mem.star`
-      hp_of (A.varray b.scs_v.slab_region) `Mem.star`
-      hp_of (A.varray b.scs_v.md_bm_region) `Mem.star`
-      hp_of (A.varray b.scs_v.md_region) `Mem.star`
-      hp_of (vptr b.scs_v.md_count)
-    ) m /\
-    sel_of (vptr r) m == b.scs_v /\
-    SL.ind_llist_sel (p_partial b.scs_v.size) b.scs_v.partial_slabs m == b.partial_slabs_v /\
-    SL.ind_llist_sel (p_empty b.scs_v.size) b.scs_v.empty_slabs m == b.empty_slabs_v /\
-    A.varrayp_sel b.scs_v.slab_region P.full_perm m == b.slab_region_v /\
-    A.varrayp_sel b.scs_v.md_bm_region P.full_perm m == b.md_bm_region_v /\
-    A.varrayp_sel b.scs_v.md_region P.full_perm m == b.md_region_v /\
-    sel_of (vptr b.scs_v.md_count) m == b.md_count_v
-  ))
-  =
-  let p1 = pts_to_sl r full_perm b.scs_v in
-  let p2 = SL.ind_llist_sl (p_partial b.scs_v.size) b.scs_v.partial_slabs in
-  let p3 = SL.ind_llist_sl (p_empty b.scs_v.size) b.scs_v.empty_slabs in
-  let p4 = hp_of (A.varray b.scs_v.slab_region) in
-  let p5 = hp_of (A.varray b.scs_v.md_bm_region) in
-  let p6 = hp_of (A.varray b.scs_v.md_region) in
-  let p7 = hp_of (vptr b.scs_v.md_count) in
-  let sl =
-    p1 `Mem.star` p2 `Mem.star` p3 `Mem.star`
-    p4 `Mem.star` p5 `Mem.star` p6 `Mem.star`
-    p7 in
-  assert (Mem.interp sl m);
-
-
-  let m123456, m7 = Mem.id_elim_star
-    (p1 `Mem.star` p2 `Mem.star` p3 `Mem.star`
-    p4 `Mem.star` p5 `Mem.star` p6)
-    p7 m in
-  let m12345, m6 = Mem.id_elim_star
-    (p1 `Mem.star` p2 `Mem.star` p3 `Mem.star` p4 `Mem.star` p5)
-    p6 m123456 in
-  let m1234, m5 = Mem.id_elim_star
-    (p1 `Mem.star` p2 `Mem.star` p3 `Mem.star` p4)
-    p5 m12345 in
-  let m123, m4 = Mem.id_elim_star
-    (p1 `Mem.star` p2 `Mem.star` p3)
-    p4 m1234 in
-  let m12, m3 = Mem.id_elim_star
-    (p1 `Mem.star` p2)
-    p3 m123 in
-  let m1, m2 = Mem.id_elim_star p1 p2 m12 in
-  // #1
-  intro_ptr_interp r b.scs_v m1;
-  ptr_sel_interp r m1;
-  pts_to_witinv r full_perm;
-  // #2-#6: empty
-  Mem.intro_star
-    (SR.ptr r) p2 m1 m2;
-  Mem.intro_star
-    (SR.ptr r `Mem.star` p2)
-    p3 m12 m3;
-  Mem.intro_star
-    (SR.ptr r `Mem.star` p2 `Mem.star` p3)
-    p4 m123 m4;
-  Mem.intro_star
-    (SR.ptr r `Mem.star` p2 `Mem.star` p3 `Mem.star` p4)
-    p5 m1234 m5;
-  Mem.intro_star
-    (SR.ptr r `Mem.star` p2 `Mem.star` p3 `Mem.star` p4 `Mem.star` p5)
-    p6 m12345 m6;
-  Mem.intro_star
-    (SR.ptr r `Mem.star` p2 `Mem.star` p3 `Mem.star` p4 `Mem.star` p5 `Mem.star` p6)
-    p7 m123456 m7
-
-#push-options "--compat_pre_typed_indexed_effects --z3rlimit 50"
-let unpack_sc (r: ref size_class_struct)
-  : Steel size_class_struct
-  (size_class_full r)
-  (fun scs ->
-    vptr r `star`
-    SL.ind_llist (p_partial scs.size) scs.partial_slabs `star`
-    SL.ind_llist (p_empty scs.size) scs.empty_slabs `star`
-    A.varray scs.slab_region `star`
-    A.varray scs.md_bm_region `star`
-    A.varray scs.md_region `star`
-    vptr scs.md_count
-  )
-  (requires fun _ -> True)
-  (ensures fun h0 scs h1 ->
-    let b = v_sc_full r h0 in
-    sel r h1 == scs /\
-    sel r h1 == b.scs_v /\
-    SL.v_ind_llist (p_partial scs.size) scs.partial_slabs h1 == b.partial_slabs_v /\
-    SL.v_ind_llist (p_empty scs.size) scs.empty_slabs h1 == b.empty_slabs_v /\
-    A.asel scs.slab_region h1 == b.slab_region_v /\
-    A.asel scs.md_bm_region h1 == b.md_bm_region_v /\
-    A.asel scs.md_region h1 == b.md_region_v /\
-    sel scs.md_count h1 == b.md_count_v
-  )
-  =
-  let h = get () in
-  let b = G.hide (v_sc_full r h) in
-  change_slprop
-    (size_class_full r)
-    (vptr r `star`
-    SL.ind_llist (p_partial b.scs_v.size) b.scs_v.partial_slabs `star`
-    SL.ind_llist (p_empty b.scs_v.size) b.scs_v.empty_slabs `star`
-    A.varray b.scs_v.slab_region `star`
-    A.varray b.scs_v.md_bm_region `star`
-    A.varray b.scs_v.md_region `star`
-    vptr b.scs_v.md_count)
-    b
-    ((((((b.scs_v,
-      b.partial_slabs_v),
-      b.empty_slabs_v),
-      b.slab_region_v),
-      b.md_bm_region_v),
-      b.md_region_v),
-      b.md_count_v)
-    (fun m -> unpack_sc_lemma r (G.reveal b) m);
-  let scs = read r in
-  change_slprop_rel
-    (SL.ind_llist (p_partial b.scs_v.size) b.scs_v.partial_slabs `star`
-    SL.ind_llist (p_empty b.scs_v.size) b.scs_v.empty_slabs `star`
-    A.varray b.scs_v.slab_region `star`
-    A.varray b.scs_v.md_bm_region `star`
-    A.varray b.scs_v.md_region `star`
-    vptr b.scs_v.md_count)
-    (SL.ind_llist (p_partial scs.size) scs.partial_slabs `star`
-    SL.ind_llist (p_empty scs.size) scs.empty_slabs `star`
-    A.varray scs.slab_region `star`
-    A.varray scs.md_bm_region `star`
-    A.varray scs.md_region `star`
-    vptr scs.md_count)
-    (fun x y -> x == y)
-    (fun _ -> ());
-  return scs
-#pop-options
-
-let pack_sc_lemma
-  (r: ref size_class_struct)
-  (b: blob2)
-  (m: Mem.mem)
-  : Lemma
-  (requires
-    Mem.interp (
-      SR.ptr r `Mem.star`
-      SL.ind_llist_sl (p_partial b.scs_v.size) b.scs_v.partial_slabs `Mem.star`
-      SL.ind_llist_sl (p_empty b.scs_v.size) b.scs_v.empty_slabs `Mem.star`
-      hp_of (A.varray b.scs_v.slab_region) `Mem.star`
-      hp_of (A.varray b.scs_v.md_bm_region) `Mem.star`
-      hp_of (A.varray b.scs_v.md_region) `Mem.star`
-      hp_of (vptr b.scs_v.md_count)
-    ) m /\
-    sel_of (vptr r) m == b.scs_v /\
-    SL.ind_llist_sel (p_partial b.scs_v.size) b.scs_v.partial_slabs m == b.partial_slabs_v /\
-    SL.ind_llist_sel (p_empty b.scs_v.size) b.scs_v.empty_slabs m == b.empty_slabs_v /\
-    A.varrayp_sel b.scs_v.slab_region P.full_perm m == b.slab_region_v /\
-    A.varrayp_sel b.scs_v.md_bm_region P.full_perm m == b.md_bm_region_v /\
-    A.varrayp_sel b.scs_v.md_region P.full_perm m == b.md_region_v /\
-    sel_of (vptr b.scs_v.md_count) m == b.md_count_v
-  )
-  (ensures
-    Mem.interp (size_class_sl r) m /\
-    size_class_sel r m == b
-  )
-  =
-  let p1 = SR.ptr r in
-  let p2 = SL.ind_llist_sl (p_partial b.scs_v.size) b.scs_v.partial_slabs in
-  let p3 = SL.ind_llist_sl (p_empty b.scs_v.size) b.scs_v.empty_slabs in
-  let p4 = hp_of (A.varray b.scs_v.slab_region) in
-  let p5 = hp_of (A.varray b.scs_v.md_bm_region) in
-  let p6 = hp_of (A.varray b.scs_v.md_region) in
-  let p7 = hp_of (vptr b.scs_v.md_count) in
-  let sl =
-    p1 `Mem.star` p2 `Mem.star` p3 `Mem.star`
-    p4 `Mem.star` p5 `Mem.star` p6 `Mem.star`
-    p7 in
-  assert (Mem.interp sl m);
-
-  let m123456, m7 = Mem.id_elim_star
-    (p1 `Mem.star` p2 `Mem.star` p3 `Mem.star` p4 `Mem.star` p5 `Mem.star` p6)
-    p7 m in
-  let m12345, m6 = Mem.id_elim_star
-    (p1 `Mem.star` p2 `Mem.star` p3 `Mem.star` p4 `Mem.star` p5)
-    p6 m123456 in
-  let m1234, m5 = Mem.id_elim_star
-    (p1 `Mem.star` p2 `Mem.star` p3 `Mem.star` p4)
-    p5 m12345 in
-  let m123, m4 = Mem.id_elim_star
-    (p1 `Mem.star` p2 `Mem.star` p3)
-    p4 m1234 in
-  let m12, m3 = Mem.id_elim_star
-    (p1 `Mem.star` p2)
-    p3 m123 in
-  let m1, m2 = Mem.id_elim_star p1 p2 m12 in
-  // #1
-  ptr_sel_interp r m1;
-  let p1' = pts_to_sl r full_perm b.scs_v in
-  // #2-#6: empty
-  Mem.intro_star
-    p1' p2 m1 m2;
-  Mem.intro_star
-    (p1' `Mem.star` p2)
-    p3 m12 m3;
-  Mem.intro_star
-    (p1' `Mem.star` p2 `Mem.star` p3)
-    p4 m123 m4;
-  Mem.intro_star
-    (p1' `Mem.star` p2 `Mem.star` p3 `Mem.star` p4)
-    p5 m1234 m5;
-  Mem.intro_star
-    (p1' `Mem.star` p2 `Mem.star` p3 `Mem.star` p4 `Mem.star` p5)
-    p6 m12345 m6;
-  Mem.intro_star
-    (p1' `Mem.star` p2 `Mem.star` p3 `Mem.star` p4 `Mem.star` p5 `Mem.star` p6)
-    p7 m123456 m7;
-  Mem.intro_h_exists b.scs_v (size_class_sl' r) m;
-  size_class_sl'_witinv r
-
-#push-options "--compat_pre_typed_indexed_effects --z3rlimit 50"
-let pack_sc (#opened:_)
-  (r: ref size_class_struct)
-  (scs: size_class_struct)
-  : SteelGhost unit opened
-  (vptr r `star`
-    SL.ind_llist (p_partial scs.size) scs.partial_slabs `star`
-    SL.ind_llist (p_empty scs.size) scs.empty_slabs `star`
-    A.varray scs.slab_region `star`
-    A.varray scs.md_bm_region `star`
-    A.varray scs.md_region `star`
-    vptr scs.md_count)
-  (fun _ -> size_class_full r)
-  (requires fun h0 -> sel r h0 == scs)
-  (ensures fun h0 _ h1 ->
-    let b = v_sc_full r h1 in
-    b.scs_v == sel r h0 /\
-    b.scs_v == scs /\
-    b.partial_slabs_v == SL.v_ind_llist (p_partial scs.size) scs.partial_slabs h0 /\
-    b.empty_slabs_v == SL.v_ind_llist (p_empty scs.size) scs.empty_slabs h0 /\
-    b.slab_region_v == A.asel scs.slab_region h0 /\
-    b.md_bm_region_v == A.asel scs.md_bm_region h0 /\
-    b.md_region_v == A.asel scs.md_region h0 /\
-    b.md_count_v == sel scs.md_count h0
-  )
-  =
-  sladmit ();
-  admit ()
-  //let h0 = get () in
-  //assert (scs == sel r h0);
-  //let partial_slabs_v : list blob
-  //  = G.hide (SL.v_ind_llist (p_partial scs.size) scs.partial_slabs h0) in
-  //let empty_slabs_v : list blob
-  //  = G.hide (SL.v_ind_llist (p_empty scs.size) scs.empty_slabs h0) in
-  //let slab_region_v : Seq.seq U8.t
-  //  = G.hide (A.asel scs.slab_region h0) in
-  //let md_bm_region_v : Seq.seq U64.t
-  //  = G.hide (A.asel scs.md_bm_region h0) in
-  //let md_region_v : Seq.seq blob
-  //  = G.hide (A.asel scs.md_region h0) in
-  //let md_count_v : U32.t
-  //  = G.hide (sel scs.md_count h0) in
-  ////let m : G.erased ((size_class_struct * list blob) * list blob) =
-  //  //G.hide ((scs, G.reveal partial_slabs_v), G.reveal empty_slabs_v) in
-  //let b : blob2 = G.hide ({
-  //  scs_v = scs;
-  //  partial_slabs_v = G.reveal partial_slabs_v;
-  //  empty_slabs_v = G.reveal empty_slabs_v;
-  //  md_count_v = G.reveal md_count_v;
-  //  slab_region_v = G.reveal slab_region_v;
-  //  md_bm_region_v = G.reveal md_bm_region_v;
-  //  md_region_v = G.reveal md_region_v;
-  //}) in
-  //change_equal_slprop
-  //  (SL.ind_llist (p_partial scs.size) scs.partial_slabs `star`
-  //  SL.ind_llist (p_empty scs.size) scs.empty_slabs `star`
-  //  A.varray scs.slab_region `star`
-  //  A.varray scs.md_bm_region `star`
-  //  A.varray scs.md_region `star`
-  //  vptr scs.md_count)
-  //  (SL.ind_llist (p_partial b.scs_v.size) b.scs_v.partial_slabs `star`
-  //  SL.ind_llist (p_empty b.scs_v.size) b.scs_v.empty_slabs `star`
-  //  A.varray b.scs_v.slab_region `star`
-  //  A.varray b.scs_v.md_bm_region `star`
-  //  A.varray b.scs_v.md_region `star`
-  //  vptr b.scs_v.md_count);
-  //change_slprop
-  //  (vptr r `star`
-  //  SL.ind_llist (p_partial b.scs_v.size) b.scs_v.partial_slabs `star`
-  //  SL.ind_llist (p_empty b.scs_v.size) b.scs_v.empty_slabs `star`
-  //  A.varray b.scs_v.slab_region `star`
-  //  A.varray b.scs_v.md_bm_region `star`
-  //  A.varray b.scs_v.md_region `star`
-  //  vptr b.scs_v.md_count)
-  //  (size_class_full r)
-  //  ((((((b.scs_v,
-  //    b.partial_slabs_v),
-  //    b.empty_slabs_v),
-  //    b.slab_region_v),
-  //    b.md_bm_region_v),
-  //    b.md_region_v),
-  //    b.md_count_v)
-  //  b
-  //  (fun m -> admit ());
-  //  //(fun m -> pack_sc_lemma r (G.reveal b) m);
-  //sladmit ();
-  //admit ()
-#pop-options
-
-let temp (r: ref size_class_struct)
-  : Steel U32.t
-  (size_class_full r)
-  (fun _ -> size_class_full r)
-  (requires fun _ -> True)
-  (ensures fun h0 _ h1 ->
-    v_sc_full r h0 == v_sc_full r h1
-  )
-  =
-  let scs = unpack_sc r in
-  pack_sc r scs;
-  return 0ul
-
-let size_class_vprop (r: ref size_class_struct)
-  =
-  SL.ind_llist (p_partial sc) partial_slabs_ptr `star`
-  SL.ind_llist (p_empty sc) empty_slabs_ptr `star`
+  SL.ind_llist (p_partial scs.size) scs.partial_slabs `star`
+  SL.ind_llist (p_empty scs.size) scs.empty_slabs `star`
   vrefinedep
-    (vptr md_count)
+    (vptr scs.md_count)
     //TODO: hideous coercion
     (fun x -> U32.v x <= U32.v metadata_max == true)
     (fun v ->
-      A.varray (A.split_r slab_region (u32_to_sz (U32.mul v page_size))) `star`
-      A.varray (A.split_r md_bm_region (u32_to_sz (U32.mul v 4ul))) `star`
-      A.varray (A.split_r md_region (u32_to_sz v)))
+      A.varray (A.split_r scs.slab_region (u32_to_sz (U32.mul v page_size))) `star`
+      A.varray (A.split_r scs.md_bm_region (u32_to_sz (U32.mul v 4ul))) `star`
+      A.varray (A.split_r scs.md_region (u32_to_sz v))
+    )
 
-(*)
-let temp2 (r: ref size_class_struct)
-  : Steel U32.t
+let size_class_vprop
+  (r: ref size_class_struct)
+  : vprop
+  =
+  vdep
+    (vptr r)
+    (fun scs -> size_class_vprop_aux scs)
+
+let size_class_vprop_test
+  (r: ref size_class_struct)
+  : Steel unit
   (size_class_vprop r)
   (fun _ -> size_class_vprop r)
-  (requires fun _ -> True)
+  (requires fun h0 -> True)
   (ensures fun h0 _ h1 ->
     h0 (size_class_vprop r)
     ==
-    h0 (size_class_vprop r)
+    h1 (size_class_vprop r)
   )
   =
-  elim_vrefine
-    (size_class_full r)
-    (fun b2 -> size_class_refinement b2);
-  let scs = unpack_sc r in
-  pack_sc r scs;
-  intro_vrefine
-    (size_class_full r)
-    (fun b2 -> size_class_refinement b2);
-  return 0ul
+  let x = elim_vdep (vptr r) (fun scs -> size_class_vprop_aux scs) in
+  intro_vdep
+    (vptr r)
+    (size_class_vprop_aux (G.reveal x))
+    (fun scs -> size_class_vprop_aux scs);
+  admit ()
 
+
+#push-options "--z3rlimit 50"
 let allocate_size_class
   (r: ref size_class_struct)
+  //: Steel unit
   : Steel (array U8.t)
   (size_class_vprop r)
   (fun result ->
@@ -544,148 +107,38 @@ let allocate_size_class
   (requires fun h0 -> True)
   (ensures fun h0 _ h1 -> True)
   =
-  elim_vrefine
-    (size_class_full r)
-    (fun b2 -> size_class_refinement b2);
-  let scs = unpack_sc r in
+  let scs' = elim_vdep
+    (vptr r)
+    (fun scs -> size_class_vprop_aux scs) in
+  let scs = read r in
+  change_slprop_rel
+    (size_class_vprop_aux (G.reveal scs'))
+    (size_class_vprop_aux scs)
+    (fun x y -> x == y)
+    (fun _ -> admit ());
+  change_slprop_rel
+    (size_class_vprop_aux scs)
+    (SL.ind_llist (p_partial scs.size) scs.partial_slabs `star`
+    SL.ind_llist (p_empty scs.size) scs.empty_slabs `star`
+    vrefinedep
+      (vptr scs.md_count)
+      //TODO: hideous coercion
+      (fun x -> U32.v x <= U32.v metadata_max == true)
+      (fun v ->
+        A.varray (A.split_r scs.slab_region (u32_to_sz (U32.mul v page_size))) `star`
+        A.varray (A.split_r scs.md_bm_region (u32_to_sz (U32.mul v 4ul))) `star`
+        A.varray (A.split_r scs.md_region (u32_to_sz v))
+      )
+    )
+    (fun x y -> x == y)
+    (fun _ -> admit ());
   let result = allocate_slab
     scs.size scs.partial_slabs scs.empty_slabs
     scs.slab_region scs.md_bm_region scs.md_region
     scs.md_count in
-  pack_sc r scs;
-  let h0 = get () in
-  let scs_v = G.hide (v_sc_full r h0) in
-  assume (size_class_refinement scs_v);
-  intro_vrefine
-    (size_class_full r)
-    (fun b2 -> size_class_refinement b2);
+  sladmit ();
+  //intro_vdep
+  //  (vptr r)
+  //  (size_class_vprop_aux scs)
+  //  (fun scs -> size_class_vprop_aux scs);
   return result
-
-(*)
-let select_size_class2 (size: U32.t)
-  (sc16 sc32 sc64: ref size_class_struct)
-  : Steel (ref size_class_struct & G.erased U32.t)
-  (size_class_full sc16 `star` size_class_full sc32 `star` size_class_full sc64)
-  (fun _ -> size_class_full sc16 `star` size_class_full sc32 `star` size_class_full sc64)
-  (requires fun h0 ->
-    (v_sc_full sc16 h0).scs_v.size == 16ul /\
-    (v_sc_full sc32 h0).scs_v.size == 32ul /\
-    (v_sc_full sc64 h0).scs_v.size == 64ul /\
-    U32.v size <= max_sc)
-  (ensures fun h0 r h1 ->
-    U32.lte size (snd r))
-  =
-
-  if U32.lte size 16ul then (
-    let sc_size = G.hide 16ul in
-    return (sc16, sc_size)
-  ) else if U32.lte size 32ul then (
-    let sc_size = G.hide 32ul in
-    return (sc32, sc_size)
-  ) else (
-    let sc_size = G.hide 64ul in
-    return (sc64, sc_size)
-  )
-
-let size_classes : list sc = [16ul ; 32ul ; 64ul]
-
-let scl_to_vprop (scl: list (ref size_class_struct))
-  : vprop
-  = starl (L.map (fun sc -> size_class_full sc) scl)
-
-let f ()
-  =
-  assert (L.memP 16ul size_classes);
-  assert_norm (L.memP 32ul size_classes);
-  assert_norm (L.memP 64ul size_classes)
-
-
-(*)
-let rec select_size_class3
-  (scl: list (ref size_class_struct))
-  (size: U32.t)
-  : Steel (ref size_class_struct)
-  (scl_to_vprop scl)
-  (fun r ->
-    size_class_full r `star`
-    scl_to_vprop (L.filter (fun r2 -> r2 =!= r) scl)
-  )
-  (requires fun h0 -> Cons? scl)
-  (ensures fun h0 r h1 ->
-    not (is_null r)
-  )
-  =
-  let r = L.hd scl in
-
-
-
-
-  admit ();
-  return null
-
-let a = 42
-(*)
-
-  (fun r ->
-    size_class_full r `star`
-    SL.ind_llist (fun sc -> size_class_full sc) size_classes)
-  (requires fun h0 ->
-    Cons? (SL.v_ind_llist (fun sc -> size_class_full sc) size_classes h0))
-  (ensures fun h0 r h1 ->
-
-  )
-
-
-
-  (size_class_full sc16 `star` size_class_full sc32 `star` size_class_full sc64)
-  (fun _ -> size_class_full sc16 `star` size_class_full sc32 `star` size_class_full sc64)
-  (requires fun h0 ->
-    (v_sc_full sc16 h0).scs_v.size == 16ul /\
-    (v_sc_full sc32 h0).scs_v.size == 32ul /\
-    (v_sc_full sc64 h0).scs_v.size == 64ul /\
-    U32.v size <= max_sc)
-  (ensures fun h0 r h1 ->
-    U32.lte size (snd r))
-  =
-
-  if U32.lte size 16ul then (
-    let sc_size = G.hide 16ul in
-    return (sc16, sc_size)
-  ) else if U32.lte size 32ul then (
-    let sc_size = G.hide 32ul in
-    return (sc32, sc_size)
-  ) else (
-    let sc_size = G.hide 64ul in
-    return (sc64, sc_size)
-  )
-
-
-
-(*)
-//noextract
-//let size_classes : list nzn = [
-//  //(* 0 *) 0;
-//  (* 16 *) 16; 32; 48; 64; 80; 96; 112; 128;
-//  (* 32 *) 160; 192; 224; 256;
-//  (* 64 *) 320; 384; 448; 512;
-//]
-//
-//
-//noextract
-//let size_class_slots : list nzn =
-//  L.map nb_of_slots size_classes
-//
-//let f (_:unit) =
-//  let v = L.nth size_class_slots 0 in
-//  assert(Some?.v v == 256);
-//  ()
-
-let page_size = 4096ul
-
-let nzn = x:U32.t{U32.v x > 0 /\ U32.v x <= U32.v page_size}
-let slab = slab:array U8.t{A.length slab == U32.v page_size}
-
-let nb_slots (x: nzn) : nzn = U32.div page_size x
-
-let slab_metadata (size_class: nzn)
-  = Seq.lseq bool (U32.v (nb_slots size_class))
